CommitmentUnpredictability.ec
@@ -3,12 +3,9 @@ require import AllCore List.
 
 type value, commitment, openingkey, message.
 
-op rndstr : (bool list) distr.
-
-op Com (x : value) (r : bool list) (m : message) : commitment * openingkey.
+op Com (pk : value) (m : message) : (commitment * openingkey) distr.
 op Ver : value -> message * (commitment * openingkey) -> bool.
 op Dpk : value distr.
-
 
 module type Guesser = {
   proc guess(pk : value) : message * (commitment * openingkey) list
@@ -19,11 +16,10 @@ module type Guesser = {
 canonically generated commitment-opening pair. *)
 module UnpredGame(G : Guesser) = {
   proc main() = {
-    var pk,m,l,c,d,rs;
+    var pk,m,l,c,d;
     pk      <$ Dpk;
-    (m , l) <- G.guess(pk); 
-    rs      <$ rndstr;
-    (c, d)  <- Com pk rs m;
+    (m, l) <- G.guess(pk); 
+    (c, d)  <$ Com pk m;
     return (c,d) \in l;
   }
 }.
